interface/Set_extended.fst
@@ -32,4 +32,3 @@ let mem_difference #a s1 s2 x = ()
 let mem_filter #a s p x = ()
 let mem_remove_x #a s x = ()
 let mem_remove_y #a s x y = ()
-          
