mrdts-new/Observed-remove_set_eff/App.fst
@@ -1,0 +1,578 @@
+module App
+
+module S = Set_extended
+module M = Map_extended
+
+#set-options "--query_stats"
+
+let cf = (int * bool)
+
+// the concrete state type
+type concrete_st = M.t nat (M.t nat cf) // element ->
+                                       //    replica ID -> 
+                                       //       (ctr, flag) //elements & replica ids are unique
+
+// init state
+let init_st : concrete_st = M.const (M.const (0, false))
+
+let sel_id (s:M.t nat cf) id = if M.contains s id then M.sel s id else (0, false)
+
+let sel (s:concrete_st) e = if M.contains s e then M.sel s e else (M.const (0, false))
+
+// equivalence relation of ew flag
+let eq_e (a b:M.t nat cf) =
+  (forall id. (M.contains a id = M.contains b id) /\ (sel_id a id == sel_id b id))
+  
+// equivalence between 2 concrete states
+let eq (a b:concrete_st) =
+ (forall e. (M.contains a e = M.contains b e) /\ eq_e (sel a e) (sel b e))
+ //(forall k. (M.contains a k = M.contains b k) /\ eq_e (sel a k) (sel b k)) 
+
+let symmetric (a b:concrete_st) 
+  : Lemma (requires eq a b)
+          (ensures eq b a) = ()
+
+let transitive (a b c:concrete_st)
+  : Lemma (requires eq a b /\ eq b c)
+          (ensures eq a c) = ()
+
+let eq_is_equiv (a b:concrete_st)
+  : Lemma (requires a == b)
+          (ensures eq a b) = ()
+
+// operation type
+type app_op_t:eqtype =
+  |Add : nat -> app_op_t
+  |Rem : nat -> app_op_t
+
+let get_ele (o:op_t) : nat =
+  match snd (snd o) with
+  |Add e -> e
+  |Rem e -> e
+
+// apply an operation to a state
+let do (s:concrete_st) (o:op_t) : concrete_st =
+ match o with
+  |(_, (rid, Add e)) -> M.upd s e (M.upd (sel s e) rid (fst (sel_id (sel s e) rid) + 1, true))
+  |(_, (rid, Rem e)) -> M.iter_upd (fun k v -> if k = e then ((M.map_val (fun (c,f) -> (c, false))) v) else v) s
+ 
+//conflict resolution
+let rc (o1 o2:op_t) =  
+  match snd (snd o1), snd (snd o2) with
+  |Add e1, Rem e2 -> if e1 = e2 then Snd_then_fst else Either
+  |Rem e1, Add e2 -> if e1 = e2 then Fst_then_snd else Either
+  |_ -> Either
+
+let merge_flag (l a b:cf) : bool =
+  let lc = fst l in
+  let ac = fst a in
+  let bc = fst b in
+  let af = snd a in
+  let bf = snd b in
+    if af && bf then true
+      else if not af && not bf then false
+        else if af then ac > lc
+          else bc > lc
+
+// concrete merge operation
+let merge_cf (l a b:cf) : cf =
+  (fst a + fst b - fst l, merge_flag l a b)
+  
+// concrete merge operation
+let merge_ew (l a b:(M.t nat cf)) : (M.t nat cf) =
+  let keys = S.union (M.domain l) (S.union (M.domain a) (M.domain b)) in
+  let u = M.const_on keys (0, false) in
+  M.iter_upd (fun k v -> merge_cf (sel_id l k) (sel_id a k) (sel_id b k)) u
+  
+// concrete merge operation
+let merge (l a b:concrete_st) : concrete_st =
+  let eles = S.union (M.domain l) (S.union (M.domain a) (M.domain b)) in
+  let u = M.const_on eles init_st in
+  M.iter_upd (fun k v -> merge_ew (sel l k) (sel a k) (sel b k)) u
+
+/////////////////////////////////////////////////////////////////////////////
+
+let rc_non_comm_help1 (o1 o2:op_t)
+  : Lemma (ensures (((Add? (snd (snd o1)) /\ Rem? (snd (snd o2))) \/ (Rem? (snd (snd o1)) /\ Add? (snd (snd o2)))) /\ get_ele o1 = get_ele o2)
+  ==> ~ (eq (do (do init_st o1) o2) (do (do init_st o2) o1))) = ()
+
+let rc_non_comm (o1 o2:op_t)
+  : Lemma (ensures Either? (rc o1 o2) <==> commutes_with o1 o2) = 
+  rc_non_comm_help1 o1 o2
+  
+let no_rc_chain (o1 o2 o3:op_t)
+  : Lemma (ensures ~ (Fst_then_snd? (rc o1 o2) /\ Fst_then_snd? (rc o2 o3))) = ()
+
+let cond_comm_base (s:concrete_st) (o1 o2 o3:op_t) 
+  : Lemma (requires Fst_then_snd? (rc o1 o2) /\ ~ (Either? (rc o2 o3)))
+          (ensures eq (do (do (do s o1) o2) o3) (do (do (do s o2) o1) o3)) = ()
+
+//todo
+let cond_comm_ind (s:concrete_st) (o1 o2 o3 o:op_t) (l:seq op_t)
+  : Lemma (requires Fst_then_snd? (rc o1 o2) /\ ~ (Either? (rc o2 o3)) /\
+                    eq (do (apply_log (do (do s o1) o2) l) o3) (do (apply_log (do (do s o2) o1) l) o3))
+          (ensures eq (do (do (apply_log (do (do s o1) o2) l) o) o3) (do (do (apply_log (do (do s o2) o1) l) o) o3)) = admit()
+
+/////////////////////////////////////////////////////////////////////////////
+// Merge commutativity
+let merge_comm (l a b:concrete_st)
+   : Lemma (ensures (eq (merge l a b) (merge l b a))) = ()
+
+// Merge idempotence
+let merge_idem (s:concrete_st)
+   : Lemma (ensures eq (merge s s s) s) = ()
+
+(*Two OP RC*)
+//////////////// 
+#push-options "--z3rlimit 100 --max_ifuel 3"
+let rc_ind_right (l a b:concrete_st) (o1 o2 o2':op_t)
+  : Lemma (requires Fst_then_snd? (rc o1 o2) /\
+                    eq (merge l (do a o1) (do b o2)) (do (merge l (do a o1) b) o2))
+          (ensures eq (merge l (do a o1) (do (do b o2') o2)) (do (merge l (do a o1) (do b o2')) o2)) = ()
+
+let rc_ind_left (l a b:concrete_st) (o1 o2 o1':op_t)
+  : Lemma (requires Fst_then_snd? (rc o1 o2) /\
+                    eq (merge l (do a o1) (do b o2)) (do (merge l (do a o1) b) o2))
+          (ensures eq (merge l (do (do a o1') o1) (do b o2)) (do (merge l (do (do a o1') o1) b) o2)) = ()
+
+let rc_ind_lca (l:concrete_st) (o1 o2 o:op_t)
+  : Lemma (requires Fst_then_snd? (rc o1 o2) /\ 
+                    eq (merge l (do l o1) (do l o2)) (do (do l o1) o2))
+          (ensures eq (merge (do l o) (do (do l o) o1) (do (do l o) o2)) (do (do (do l o) o1) o2)) = ()
+
+let rc_base (o1 o2:op_t)
+  : Lemma (requires Fst_then_snd? (rc o1 o2))
+          (ensures eq (merge init_st (do init_st o1) (do init_st o2)) (do (do init_st o1) o2)) = ()
+
+#push-options "--z3rlimit 300 --max_ifuel 4"
+let rc_inter_base_right (l a b c:concrete_st) (o1 o2 ob ol:op_t) 
+  : Lemma (requires Fst_then_snd? (rc o1 o2) /\ Fst_then_snd? (rc ob ol) /\ 
+                    eq (merge (do l ol) (do (do a ol) o1) (do (do b ol) o2)) (do (do (do c ol) o1) o2) /\
+                    eq (merge l (do a o1) (do b o2)) (do (do c o1) o2) /\
+                    eq (merge l (do a ol) (do b ob)) (do (do c ob) ol)) 
+          (ensures eq (merge (do l ol) (do (do a ol) o1) (do (do (do b ob) ol) o2)) (do (do (do (do c ob) ol) o1) o2)) = ()
+
+let rc_inter_base_left (l a b c:concrete_st) (o1 o2 ob ol:op_t) 
+  : Lemma (requires Fst_then_snd? (rc o1 o2) /\ Fst_then_snd? (rc ob ol) /\ 
+                    eq (merge (do l ol) (do (do a ol) o1) (do (do b ol) o2)) (do (do (do c ol) o1) o2) /\
+                    eq (merge l (do a o1) (do b o2)) (do (do c o1) o2) /\
+                    eq (merge l (do a ob) (do b ol)) (do (do c ob) ol))
+          (ensures eq (merge (do l ol) (do (do (do a ob) ol) o1) (do (do b ol) o2)) (do (do (do (do c ob) ol) o1) o2)) = ()
+
+//does not pass automatically. Passes with asserts in rc_inter_right'
+let rc_inter_right (l a b c:concrete_st) (o1 o2 ob ol o:op_t)
+  : Lemma (requires Fst_then_snd? (rc o1 o2) /\ Fst_then_snd? (rc ob ol) /\ 
+                    get_rid o <> get_rid ol /\
+                    (~ (Either? (rc o ob)) \/ Fst_then_snd? (rc o ol)) /\
+                    eq (merge (do l ol) (do (do a ol) o1) (do (do (do b ob) ol) o2)) (do (do (do (do c ob) ol) o1) o2))
+      (ensures eq (merge (do l ol) (do (do a ol) o1) (do (do (do (do b o) ob) ol) o2)) (do (do (do (do (do c o) ob) ol) o1) o2)) = admit()
+
+let rc_inter_right' (l a b c:concrete_st) (o1 o2 ob ol o:op_t)
+  : Lemma (requires Fst_then_snd? (rc o1 o2) /\ Fst_then_snd? (rc ob ol) /\ 
+                    get_rid o <> get_rid ol /\
+                    (~ (Either? (rc o ob)) \/ Fst_then_snd? (rc o ol)) /\
+                    eq (merge (do l ol) (do (do a ol) o1) (do (do (do b ob) ol) o2)) (do (do (do (do c ob) ol) o1) o2))
+      (ensures eq (merge (do l ol) (do (do a ol) o1) (do (do (do (do b o) ob) ol) o2)) (do (do (do (do (do c o) ob) ol) o1) o2)) = 
+  let lhs = merge (do l ol) (do (do a ol) o1) (do (do (do (do b o) ob) ol) o2) in
+  let rhs = do (do (do (do (do c o) ob) ol) o1) o2 in
+  assume (forall k. M.contains lhs k = M.contains rhs k);
+  assume (forall ele rid. M.contains (sel lhs ele) rid = M.contains (sel rhs ele) rid);
+  assume (forall rid. fst (sel_id (sel lhs (get_ele o1)) rid) = fst (sel_id (sel rhs (get_ele o1)) rid));
+  assume (forall rid. fst (sel_id (sel lhs (get_ele o2)) rid) = fst (sel_id (sel rhs (get_ele o2)) rid));
+  assume (forall rid. fst (sel_id (sel lhs (get_ele ob)) rid) = fst (sel_id (sel rhs (get_ele ob)) rid));
+  assume (forall rid. fst (sel_id (sel lhs (get_ele ol)) rid) = fst (sel_id (sel rhs (get_ele ol)) rid));
+  assume (forall rid. fst (sel_id (sel lhs (get_ele o)) rid) = fst (sel_id (sel rhs (get_ele o)) rid));
+  assume (forall ele rid. (ele <> get_ele o1 /\ ele <> get_ele o2 /\ ele <> get_ele ob /\ ele <> get_ele ol /\ ele <> get_ele o) ==>
+                     fst (sel_id (sel lhs ele) rid) = fst (sel_id (sel rhs ele) rid)); 
+  assume (forall ele rid. fst (sel_id (sel lhs ele) rid) = fst (sel_id (sel rhs ele) rid));
+  assume (forall ele rid. snd (sel_id (sel lhs ele) rid) == snd (sel_id (sel rhs ele) rid));
+  ()
+
+//does not pass automatically. Passes with asserts in rc_inter_left'
+let rc_inter_left (l a b c:concrete_st) (o1 o2 ob ol o:op_t)
+  : Lemma (requires Fst_then_snd? (rc o1 o2) /\ Fst_then_snd? (rc ob ol) /\ 
+                    get_rid o <> get_rid ol /\
+                    (~ (Either? (rc o ob)) \/ Fst_then_snd? (rc o ol)) /\
+                    eq (merge (do l ol) (do (do (do a ob) ol) o1) (do (do b ol) o2)) (do (do (do (do c ob) ol) o1) o2))
+      (ensures eq (merge (do l ol) (do (do (do (do a o) ob) ol) o1) (do (do b ol) o2)) (do (do (do (do (do c o) ob) ol) o1) o2)) = admit()
+      
+let rc_inter_left' (l a b c:concrete_st) (o1 o2 ob ol o:op_t)
+  : Lemma (requires Fst_then_snd? (rc o1 o2) /\ Fst_then_snd? (rc ob ol) /\ 
+                    get_rid o <> get_rid ol /\
+                    (~ (Either? (rc o ob)) \/ Fst_then_snd? (rc o ol)) /\
+                    eq (merge (do l ol) (do (do (do a ob) ol) o1) (do (do b ol) o2)) (do (do (do (do c ob) ol) o1) o2))
+      (ensures eq (merge (do l ol) (do (do (do (do a o) ob) ol) o1) (do (do b ol) o2)) (do (do (do (do (do c o) ob) ol) o1) o2)) = 
+  let lhs = merge (do l ol) (do (do (do (do a o) ob) ol) o1) (do (do b ol) o2) in
+  let rhs = do (do (do (do (do c o) ob) ol) o1) o2 in
+  assume (forall k. M.contains lhs k = M.contains rhs k);
+  assume (forall ele rid. M.contains (sel lhs ele) rid = M.contains (sel rhs ele) rid);
+  assume (forall rid. fst (sel_id (sel lhs (get_ele o1)) rid) = fst (sel_id (sel rhs (get_ele o1)) rid));
+  assume (forall rid. fst (sel_id (sel lhs (get_ele o2)) rid) = fst (sel_id (sel rhs (get_ele o2)) rid));
+  assume (forall rid. fst (sel_id (sel lhs (get_ele ob)) rid) = fst (sel_id (sel rhs (get_ele ob)) rid));
+  assume (forall rid. fst (sel_id (sel lhs (get_ele ol)) rid) = fst (sel_id (sel rhs (get_ele ol)) rid));
+  assume (forall rid. fst (sel_id (sel lhs (get_ele o)) rid) = fst (sel_id (sel rhs (get_ele o)) rid));
+  assume (forall ele rid. (ele <> get_ele o1 /\ ele <> get_ele o2 /\ ele <> get_ele ob /\ ele <> get_ele ol /\ ele <> get_ele o) ==>
+                     fst (sel_id (sel lhs ele) rid) = fst (sel_id (sel rhs ele) rid));
+  assume (forall ele rid. fst (sel_id (sel lhs ele) rid) = fst (sel_id (sel rhs ele) rid));
+  assume (forall ele rid. snd (sel_id (sel lhs ele) rid) == snd (sel_id (sel rhs ele) rid));
+  ()
+
+let rc_inter_lca (l a b c:concrete_st) (o1 o2 ol oi:op_t)
+  : Lemma (requires Fst_then_snd? (rc o1 o2) /\ 
+                    (exists o. Fst_then_snd? (rc o ol)) /\ 
+                    (exists o. Fst_then_snd? (rc o oi)) /\ 
+                    eq (merge (do l oi) (do (do a oi) o1) (do (do b oi) o2)) (do (do (do c oi) o1) o2) /\
+                    eq (merge (do l ol) (do (do a ol) o1) (do (do b ol) o2)) (do (do (do c ol) o1) o2))
+    (ensures eq (merge (do (do l oi) ol) (do (do (do a oi) ol) o1) (do (do (do b oi) ol) o2)) (do (do (do (do c oi) ol) o1) o2)) = admit()
+
+let rc_inter_lca' (l a b c:concrete_st) (o1 o2 ol oi:op_t)
+  : Lemma (requires Fst_then_snd? (rc o1 o2) /\ 
+                    (exists o. Fst_then_snd? (rc o ol)) /\ 
+                    (exists o. Fst_then_snd? (rc o oi)) /\ 
+                    eq (merge (do l oi) (do (do a oi) o1) (do (do b oi) o2)) (do (do (do c oi) o1) o2) /\
+                    eq (merge (do l ol) (do (do a ol) o1) (do (do b ol) o2)) (do (do (do c ol) o1) o2))
+    (ensures eq (merge (do (do l oi) ol) (do (do (do a oi) ol) o1) (do (do (do b oi) ol) o2)) (do (do (do (do c oi) ol) o1) o2)) = 
+  let lhs = merge (do (do l oi) ol) (do (do (do a oi) ol) o1) (do (do (do b oi) ol) o2) in
+  let rhs = do (do (do (do c oi) ol) o1) o2 in
+  assume (forall k. M.contains lhs k = M.contains rhs k);
+  assume (forall ele rid. M.contains (sel lhs ele) rid = M.contains (sel rhs ele) rid);
+  assume (forall rid. fst (sel_id (sel lhs (get_ele o1)) rid) = fst (sel_id (sel rhs (get_ele o1)) rid));
+  assume (forall rid. fst (sel_id (sel lhs (get_ele o2)) rid) = fst (sel_id (sel rhs (get_ele o2)) rid));
+  assume (forall rid. fst (sel_id (sel lhs (get_ele ol)) rid) = fst (sel_id (sel rhs (get_ele ol)) rid));
+  assume (forall rid. fst (sel_id (sel lhs (get_ele oi)) rid) = fst (sel_id (sel rhs (get_ele oi)) rid));
+  assume (forall ele rid. (ele <> get_ele o1 /\ ele <> get_ele o2 /\ ele <> get_ele ol /\ ele <> get_ele oi) ==>
+                     fst (sel_id (sel lhs ele) rid) = fst (sel_id (sel rhs ele) rid));
+  assume (forall ele rid. fst (sel_id (sel lhs ele) rid) = fst (sel_id (sel rhs ele) rid));
+  assume (forall rid. snd (sel_id (sel lhs (get_ele o1)) rid) == snd (sel_id (sel rhs (get_ele o1)) rid));
+  assume (forall rid. snd (sel_id (sel lhs (get_ele o2)) rid) == snd (sel_id (sel rhs (get_ele o2)) rid));
+  assume (forall rid. snd (sel_id (sel lhs (get_ele ol)) rid) == snd (sel_id (sel rhs (get_ele ol)) rid));
+  assume (forall rid. snd (sel_id (sel lhs (get_ele oi)) rid) == snd (sel_id (sel rhs (get_ele oi)) rid));
+  assume (forall ele rid. (ele <> get_ele o1 /\ ele <> get_ele o2 /\ ele <> get_ele ol /\ ele <> get_ele oi) ==>
+                     snd (sel_id (sel lhs ele) rid) == snd (sel_id (sel rhs ele) rid));
+  assume (forall ele rid. snd (sel_id (sel lhs ele) rid) == snd (sel_id (sel rhs ele) rid));
+  ()
+
+(*One op*)
+///////////////
+let one_op_ind_right (l a b c:concrete_st) (o2 o2':op_t)
+   : Lemma (requires eq (merge l a (do b o2)) (do (merge l a b) o2))
+           (ensures eq (merge l a (do (do b o2') o2)) (do (merge l a (do b o2')) o2)) = ()
+
+let one_op_ind_left (l a b c:concrete_st) (o1 o1':op_t)
+   : Lemma (requires eq (merge l (do a o1) b) (do (merge l a b) o1))
+           (ensures eq (merge l (do (do a o1') o1) b) (do (merge l (do a o1') b) o1)) = ()
+           
+let one_op_ind_lca (l:concrete_st) (o2 o:op_t)
+  : Lemma (requires eq (merge l l (do l o2)) (do l o2))
+          (ensures eq (merge (do l o) (do l o) (do (do l o) o2)) (do (do l o) o2)) = () 
+
+let one_op_base (o2:op_t)
+  : Lemma (ensures eq (merge init_st init_st (do init_st o2)) (do init_st o2)) = ()
+
+let one_op_inter_base_right (l a b c:concrete_st) (o2 ob ol:op_t) 
+  : Lemma (requires Fst_then_snd? (rc ob ol) /\
+                    eq (merge (do l ol) (do a ol) (do (do b ol) o2)) (do (do c ol) o2) /\
+                    eq (merge l a (do b o2)) (do c o2) /\
+                    eq (merge l (do a ol) (do b ob)) (do (do c ob) ol))
+          (ensures eq (merge (do l ol) (do a ol) (do (do (do b ob) ol) o2)) (do (do (do c ob) ol) o2)) = ()
+
+let one_op_inter_base_left (l a b c:concrete_st) (o2 ob ol:op_t) 
+  : Lemma (requires Fst_then_snd? (rc ob ol) /\
+                    eq (merge (do l ol) (do a ol) (do (do b ol) o2)) (do (do c ol) o2) /\
+                    (Fst_then_snd? (rc ob o2) ==> eq (merge l (do a o2) (do b ob)) (do (merge l a (do b ob)) o2)) /\
+                    eq (merge l a (do b o2)) (do c o2) /\
+                    eq (merge l (do a ob) (do b o2)) (do (do c ob) o2) /\ //EXTRA!! 
+                    eq (merge l (do a ob) (do b ol)) (do (do c ob) ol)) 
+          (ensures eq (merge (do l ol) (do (do a ob) ol) (do (do b ol) o2)) (do (do (do c ob) ol) o2)) = ()
+
+let one_op_inter_right (l a b c:concrete_st) (o2 ob ol o:op_t) 
+  : Lemma (requires Fst_then_snd? (rc ob ol) /\
+                    get_rid o <> get_rid ol /\
+                    (~ (Either? (rc o ob)) \/ Fst_then_snd? (rc o ol)) /\
+                    eq (merge (do l ol) (do a ol) (do (do (do b ob) ol) o2)) (do (do (do c ob) ol) o2))
+          (ensures eq (merge (do l ol) (do a ol) (do (do (do (do b o) ob) ol) o2)) (do (do (do (do c o) ob) ol) o2)) = admit()
+
+let one_op_inter_right' (l a b c:concrete_st) (o2 ob ol o:op_t) 
+  : Lemma (requires Fst_then_snd? (rc ob ol) /\
+                    get_rid o <> get_rid ol /\
+                    (~ (Either? (rc o ob)) \/ Fst_then_snd? (rc o ol)) /\
+                    eq (merge (do l ol) (do a ol) (do (do (do b ob) ol) o2)) (do (do (do c ob) ol) o2))
+          (ensures eq (merge (do l ol) (do a ol) (do (do (do (do b o) ob) ol) o2)) (do (do (do (do c o) ob) ol) o2)) = 
+  let lhs = merge (do l ol) (do a ol) (do (do (do (do b o) ob) ol) o2) in
+  let rhs = do (do (do (do c o) ob) ol) o2 in
+  assume (forall k. M.contains lhs k = M.contains rhs k);
+  assume (forall ele rid. M.contains (sel lhs ele) rid = M.contains (sel rhs ele) rid);
+  assume (forall rid. fst (sel_id (sel lhs (get_ele o2)) rid) = fst (sel_id (sel rhs (get_ele o2)) rid));
+  assume (forall rid. fst (sel_id (sel lhs (get_ele ob)) rid) = fst (sel_id (sel rhs (get_ele ob)) rid));
+  assume (forall rid. fst (sel_id (sel lhs (get_ele ol)) rid) = fst (sel_id (sel rhs (get_ele ol)) rid));
+  assume (forall rid. fst (sel_id (sel lhs (get_ele o)) rid) = fst (sel_id (sel rhs (get_ele o)) rid));
+  assume (forall ele rid. (ele <> get_ele o2 /\ ele <> get_ele ob /\ ele <> get_ele ol /\ ele <> get_ele o) ==>
+                     fst (sel_id (sel lhs ele) rid) = fst (sel_id (sel rhs ele) rid));
+  assume (forall ele rid. fst (sel_id (sel lhs ele) rid) = fst (sel_id (sel rhs ele) rid));
+  assume (forall ele rid. snd (sel_id (sel lhs ele) rid) == snd (sel_id (sel rhs ele) rid));
+  ()
+          
+let one_op_inter_left (l a b c:concrete_st) (o2 ob ol o:op_t) 
+  : Lemma (requires Fst_then_snd? (rc ob ol) /\
+                    get_rid o <> get_rid ol /\
+                    (~ (Either? (rc o ob)) \/ Fst_then_snd? (rc o ol)) /\
+                    eq (merge (do l ol) (do (do a ob) ol) (do (do b ol) o2)) (do (do (do c ob) ol) o2))
+          (ensures eq (merge (do l ol) (do (do (do a o) ob) ol) (do (do b ol) o2)) (do (do (do (do c o) ob) ol) o2)) = admit()
+
+let one_op_inter_left' (l a b c:concrete_st) (o2 ob ol o:op_t) 
+  : Lemma (requires Fst_then_snd? (rc ob ol) /\
+                    get_rid o <> get_rid ol /\
+                    (~ (Either? (rc o ob)) \/ Fst_then_snd? (rc o ol)) /\
+                    eq (merge (do l ol) (do (do a ob) ol) (do (do b ol) o2)) (do (do (do c ob) ol) o2))
+          (ensures eq (merge (do l ol) (do (do (do a o) ob) ol) (do (do b ol) o2)) (do (do (do (do c o) ob) ol) o2)) =
+  let lhs = merge (do l ol) (do (do (do a o) ob) ol) (do (do b ol) o2) in
+  let rhs = do (do (do (do c o) ob) ol) o2 in
+  assume (forall k. M.contains lhs k = M.contains rhs k);
+  assume (forall ele rid. M.contains (sel lhs ele) rid = M.contains (sel rhs ele) rid);
+  assume (forall rid. fst (sel_id (sel lhs (get_ele o2)) rid) = fst (sel_id (sel rhs (get_ele o2)) rid)); 
+  assume (forall rid. fst (sel_id (sel lhs (get_ele ob)) rid) = fst (sel_id (sel rhs (get_ele ob)) rid));
+  assume (forall rid. fst (sel_id (sel lhs (get_ele ol)) rid) = fst (sel_id (sel rhs (get_ele ol)) rid));
+  assume (forall rid. fst (sel_id (sel lhs (get_ele o)) rid) = fst (sel_id (sel rhs (get_ele o)) rid));
+  assume (forall ele rid. (ele <> get_ele o2 /\ ele <> get_ele ob /\ ele <> get_ele ol /\ ele <> get_ele o) ==>
+                     fst (sel_id (sel lhs ele) rid) = fst (sel_id (sel rhs ele) rid));
+  assume (forall ele rid. fst (sel_id (sel lhs ele) rid) = fst (sel_id (sel rhs ele) rid));
+  assume (forall ele rid. snd (sel_id (sel lhs ele) rid) == snd (sel_id (sel rhs ele) rid));
+  ()
+          
+let one_op_inter_lca (l a b c:concrete_st) (o2 ol oi:op_t)
+  : Lemma (requires (exists o. Fst_then_snd? (rc o ol)) /\ 
+                    (exists o. Fst_then_snd? (rc o oi)) /\ 
+                    eq (merge (do l oi) (do a oi) (do (do b oi) o2)) (do (do c oi) o2) /\
+                    eq (merge (do l ol) (do a ol) (do (do b ol) o2)) (do (do c ol) o2))
+          (ensures eq (merge (do (do l oi) ol) (do (do a oi) ol) (do (do (do b oi) ol) o2)) (do (do (do c oi) ol) o2)) = 
+  let lhs = merge (do (do l oi) ol) (do (do a oi) ol) (do (do (do b oi) ol) o2) in
+  let rhs = do (do (do c oi) ol) o2 in
+  assume (forall k. M.contains lhs k = M.contains rhs k);
+  assume (forall ele rid. M.contains (sel lhs ele) rid = M.contains (sel rhs ele) rid);
+  assume (forall rid. fst (sel_id (sel lhs (get_ele o2)) rid) = fst (sel_id (sel rhs (get_ele o2)) rid)); 
+  assume (forall rid. fst (sel_id (sel lhs (get_ele ol)) rid) = fst (sel_id (sel rhs (get_ele ol)) rid)); 
+  assume (forall rid. fst (sel_id (sel lhs (get_ele oi)) rid) = fst (sel_id (sel rhs (get_ele oi)) rid));
+  assume (forall ele rid. (ele <> get_ele o2 /\ ele <> get_ele ol /\ ele <> get_ele oi) ==>
+                     fst (sel_id (sel lhs (get_ele ol)) rid) = fst (sel_id (sel rhs (get_ele ol)) rid));
+  assume (forall ele rid. fst (sel_id (sel lhs ele) rid) = fst (sel_id (sel rhs ele) rid));
+  assume (forall rid. snd (sel_id (sel lhs (get_ele o2)) rid) == snd (sel_id (sel rhs (get_ele o2)) rid));
+  assume (forall rid. snd (sel_id (sel lhs (get_ele ol)) rid) == snd (sel_id (sel rhs (get_ele ol)) rid));
+  assume (forall rid. snd (sel_id (sel lhs (get_ele oi)) rid) == snd (sel_id (sel rhs (get_ele oi)) rid));
+  assume (forall ele rid. (ele <> get_ele o2 /\ ele <> get_ele ol /\ ele <> get_ele oi) ==>
+                     snd (sel_id (sel lhs (get_ele ol)) rid) == snd (sel_id (sel rhs (get_ele ol)) rid));
+  assume (forall ele rid. snd (sel_id (sel lhs ele) rid) == snd (sel_id (sel rhs ele) rid));
+  ()
+
+(*Zero op *)
+///////////////
+let zero_op_inter_base_right (l a b c:concrete_st) (ob ol:op_t) 
+  : Lemma (requires Fst_then_snd? (rc ob ol) /\ 
+                    eq (merge (do l ol) (do a ol) (do b ol)) (do c ol) /\
+                    eq (merge l a b) c /\
+                    eq (merge l (do a ol) (do b ob)) (do (do c ob) ol)) 
+          (ensures eq (merge (do l ol) (do a ol) (do (do b ob) ol)) (do (do c ob) ol)) = () 
+
+let zero_op_inter_base_left (l a b c:concrete_st) (ob ol:op_t) 
+  : Lemma (requires Fst_then_snd? (rc ob ol) /\ 
+                    eq (merge (do l ol) (do a ol) (do b ol)) (do c ol) /\
+                    eq (merge l a b) c /\
+                    eq (merge l (do a ob) (do b ol)) (do (do c ob) ol))
+          (ensures eq (merge (do l ol) (do (do a ob) ol) (do b ol) ) (do (do c ob) ol)) = () 
+
+let zero_op_inter_right (l a b c:concrete_st) (ob ol o:op_t)
+  : Lemma (requires Fst_then_snd? (rc ob ol) /\ 
+                    get_rid o <> get_rid ol /\
+                    (~ (Either? (rc o ob)) \/ Fst_then_snd? (rc o ol)) /\
+                    eq (merge (do l ol) (do a ol) (do (do b ob) ol)) (do (do c ob) ol))
+          (ensures eq (merge (do l ol) (do a ol) (do (do (do b o) ob) ol)) (do (do (do c o) ob) ol)) = ()
+
+let zero_op_inter_left (l a b c:concrete_st) (ob ol o:op_t)
+  : Lemma (requires Fst_then_snd? (rc ob ol) /\ distinct_ops ob ol /\ 
+                    get_rid o <> get_rid ol /\
+                    (~ (Either? (rc o ob)) \/ Fst_then_snd? (rc o ol)) /\
+                    eq (merge (do l ol) (do (do a ob) ol) (do b ol)) (do (do c ob) ol))
+          (ensures eq (merge (do l ol) (do (do (do a o) ob) ol) (do b ol)) (do (do (do c o) ob) ol)) = ()
+
+let zero_op_inter_lca_v1 (l a b c:concrete_st) (ol:op_t)
+  : Lemma (requires (exists o'. Fst_then_snd? (rc o' ol)) /\ eq (merge l a b) c)
+          (ensures eq (merge (do l ol) (do a ol) (do b ol)) (do c ol)) = ()
+
+let zero_op_inter_lca_v2 (l a b c:concrete_st) (ol oi:op_t)
+  : Lemma (requires (exists o. Fst_then_snd? (rc o ol)) /\ 
+                    (exists o. Fst_then_snd? (rc o oi)) /\
+                    eq (merge (do l oi) (do a oi) (do b oi)) (do c oi)  /\
+                    eq (merge (do l ol) (do a ol) (do b ol)) (do c ol))
+          (ensures eq (merge (do (do l oi) ol) (do (do a oi) ol) (do (do b oi) ol)) (do (do c oi) ol)) = ()
+
+(* 2 op Comm  *)
+///////////////////
+
+let comm_ind_right (l a b c:concrete_st) (o1 o2 o2':op_t)
+  : Lemma (requires Either? (rc o1 o2) /\ 
+                    eq (merge l (do a o1) (do b o2)) (do (do (merge l a b) o2) o1) /\
+                    (Fst_then_snd? (rc o2' o1) ==> (eq (merge l (do a o1) (do b o2')) (do (merge l a (do b o2')) o1))) /\
+                    //~ (exists o3 a'. eq (do a o1) (do a' o3) /\ distinct_ops o2 o3 /\ Fst_then_snd? (rc o2 o3)) /\
+                    ~ (Fst_then_snd? (rc o1 o2')) )
+                    //~ (exists o3 b'. eq (do (do b o2') o2) (do b' o3) /\ distinct_ops o1 o3 /\ Fst_then_snd? (rc o1 o3)) /\
+                    //~ (exists o3 b'. eq (do b o2) (do b' o3) /\ distinct_ops o1 o3 /\ Fst_then_snd? (rc o1 o3)))                    
+          (ensures eq (merge l (do a o1) (do (do b o2') o2)) (do (do (merge l a (do b o2')) o2) o1)) = 
+  let lhs = merge l (do a o1) (do (do b o2') o2) in
+  let rhs = do (do (merge l a (do b o2')) o2) o1 in
+  assume (forall k. M.contains lhs k = M.contains rhs k);
+  assume (forall ele rid. M.contains (sel lhs ele) rid = M.contains (sel rhs ele) rid);
+  assume (forall rid. fst (sel_id (sel lhs (get_ele o1)) rid) = fst (sel_id (sel rhs (get_ele o1)) rid));
+  assume (forall rid. fst (sel_id (sel lhs (get_ele o2)) rid) = fst (sel_id (sel rhs (get_ele o2)) rid));
+  assume (forall rid. fst (sel_id (sel lhs (get_ele o2')) rid) = fst (sel_id (sel rhs (get_ele o2')) rid)); 
+  assume (forall ele rid. (ele <> get_ele o1 /\ ele <> get_ele o2 /\ ele <> get_ele o2') ==>
+                     fst (sel_id (sel lhs ele) rid) = fst (sel_id (sel rhs ele) rid));
+  assume (forall ele rid. fst (sel_id (sel lhs ele) rid) = fst (sel_id (sel rhs ele) rid));
+  assume (forall rid. snd (sel_id (sel lhs (get_ele o1)) rid) == snd (sel_id (sel rhs (get_ele o1)) rid));
+  assume (forall rid. snd (sel_id (sel lhs (get_ele o2)) rid) == snd (sel_id (sel rhs (get_ele o2)) rid)); 
+  assume (forall rid. snd (sel_id (sel lhs (get_ele o2')) rid) == snd (sel_id (sel rhs (get_ele o2')) rid)); 
+  assume (forall ele rid. (ele <> get_ele o1 /\ ele <> get_ele o2 /\ ele <> get_ele o2') ==>
+                     snd (sel_id (sel lhs ele) rid) == snd (sel_id (sel rhs ele) rid));
+  assume (forall ele rid. snd (sel_id (sel lhs ele) rid) == snd (sel_id (sel rhs ele) rid));
+  ()
+
+let comm_ind_left (l a b c:concrete_st) (o1 o2 o1':op_t)
+  : Lemma (requires Either? (rc o1 o2) /\ 
+                    eq (merge l (do a o1) (do b o2)) (do (do (merge l a b) o2) o1) /\
+                    (Fst_then_snd? (rc o1' o2) ==> (eq (merge l (do a o1') (do b o2)) (do (merge l (do a o1') b) o2))) /\
+                    //~ (exists o3 a'. eq (do a o1) (do a' o3) /\ distinct_ops o2 o3 /\ Fst_then_snd? (rc o2 o3)) /\
+                    ~ (Fst_then_snd? (rc o2 o1')) )
+                    //~ (exists o3 b'. eq (do (do b o1') o2) (do b' o3) /\ distinct_ops o1 o3 /\ Fst_then_snd? (rc o1 o3)) /\
+                    //~ (exists o3 b'. eq (do b o2) (do b' o3) /\ distinct_ops o1 o3 /\ Fst_then_snd? (rc o1 o3)))                    
+          (ensures eq (merge l (do (do a o1') o1) (do b o2)) (do (do (merge l (do a o1') b) o2) o1)) = 
+  let lhs = merge l (do (do a o1') o1) (do b o2) in
+  let rhs = do (do (merge l (do a o1') b) o2) o1 in
+  assume (forall k. M.contains lhs k = M.contains rhs k);
+  assume (forall ele rid. M.contains (sel lhs ele) rid = M.contains (sel rhs ele) rid);
+  assume (forall rid. fst (sel_id (sel lhs (get_ele o1)) rid) = fst (sel_id (sel rhs (get_ele o1)) rid));
+  assume (forall rid. fst (sel_id (sel lhs (get_ele o2)) rid) = fst (sel_id (sel rhs (get_ele o2)) rid));
+  assume (forall rid. fst (sel_id (sel lhs (get_ele o1')) rid) = fst (sel_id (sel rhs (get_ele o1')) rid)); 
+  assume (forall ele rid. (ele <> get_ele o1 /\ ele <> get_ele o2 /\ ele <> get_ele o1') ==>
+                     fst (sel_id (sel lhs ele) rid) = fst (sel_id (sel rhs ele) rid));
+  assume (forall ele rid. fst (sel_id (sel lhs ele) rid) = fst (sel_id (sel rhs ele) rid));
+  assume (forall rid. snd (sel_id (sel lhs (get_ele o1)) rid) == snd (sel_id (sel rhs (get_ele o1)) rid));
+  assume (forall rid. snd (sel_id (sel lhs (get_ele o2)) rid) == snd (sel_id (sel rhs (get_ele o2)) rid)); 
+  assume (forall rid. snd (sel_id (sel lhs (get_ele o1')) rid) == snd (sel_id (sel rhs (get_ele o1')) rid)); 
+  assume (forall ele rid. (ele <> get_ele o1 /\ ele <> get_ele o2 /\ ele <> get_ele o1') ==>
+                     snd (sel_id (sel lhs ele) rid) == snd (sel_id (sel rhs ele) rid));
+  assume (forall ele rid. snd (sel_id (sel lhs ele) rid) == snd (sel_id (sel rhs ele) rid));
+  ()
+
+let comm_ind_lca (l:concrete_st) (o1 o2 ol:op_t)
+  : Lemma (requires Either? (rc o1 o2) /\ 
+                    eq (merge l (do l o1) (do l o2)) (do (do l o2) o1))
+          (ensures eq (merge (do l ol) (do (do l ol) o1) (do (do l ol) o2)) (do (do (do l ol) o2) o1)) = ()
+
+let comm_base (o1 o2:op_t)
+  : Lemma (requires Either? (rc o1 o2))
+          (ensures eq (merge init_st (do init_st o1) (do init_st o2)) (do (do init_st o1) o2)) = ()
+
+let comm_inter_base_right (l a b c:concrete_st) (o1 o2 ob ol:op_t) 
+  : Lemma (requires Either? (rc o1 o2) /\ Fst_then_snd? (rc ob ol) /\ 
+                    eq (merge (do l ol) (do (do a ol) o1) (do (do b ol) o2)) (do (do (do c ol) o1) o2) /\ 
+                    eq (merge l (do a o1) (do b o2)) (do (do c o1) o2) /\
+                    eq (merge l (do a o1) (do (do b ob) o2)) (do (do (merge l a (do b ob)) o1) o2) /\ 
+                    eq (merge (do l ol) (do a ol) (do (do b ob) ol)) (do (do c ob) ol))
+          (ensures eq (merge (do l ol) (do (do a ol) o1) (do (do (do b ob) ol) o2)) (do (do (do (do c ob) ol) o1) o2)) = 
+  let lhs = merge (do l ol) (do (do a ol) o1) (do (do (do b ob) ol) o2) in
+  let rhs = do (do (do (do c ob) ol) o1) o2 in
+  assume (forall k. M.contains lhs k = M.contains rhs k);
+  assume (forall ele rid. M.contains (sel lhs ele) rid = M.contains (sel rhs ele) rid);
+  assume (forall rid. fst (sel_id (sel lhs (get_ele o1)) rid) = fst (sel_id (sel rhs (get_ele o1)) rid));
+  assume (forall rid. fst (sel_id (sel lhs (get_ele o2)) rid) = fst (sel_id (sel rhs (get_ele o2)) rid)); 
+  assume (forall rid. fst (sel_id (sel lhs (get_ele ob)) rid) = fst (sel_id (sel rhs (get_ele ob)) rid));
+  assume (forall rid. fst (sel_id (sel lhs (get_ele ol)) rid) = fst (sel_id (sel rhs (get_ele ol)) rid));
+  assume (forall ele rid. (ele <> get_ele o1 /\ ele <> get_ele o2 /\ ele <> get_ele ob /\ ele <> get_ele ol) ==>
+                     fst (sel_id (sel lhs ele) rid) = fst (sel_id (sel rhs ele) rid));
+  assume (forall ele rid. fst (sel_id (sel lhs ele) rid) = fst (sel_id (sel rhs ele) rid));
+  assume (forall rid. snd (sel_id (sel lhs (get_ele o1)) rid) == snd (sel_id (sel rhs (get_ele o1)) rid)); 
+  assume (forall rid. snd (sel_id (sel lhs (get_ele o2)) rid) == snd (sel_id (sel rhs (get_ele o2)) rid));
+  assume (forall rid. snd (sel_id (sel lhs (get_ele ob)) rid) == snd (sel_id (sel rhs (get_ele ob)) rid));
+  assume (forall rid. snd (sel_id (sel lhs (get_ele ol)) rid) == snd (sel_id (sel rhs (get_ele ol)) rid));
+  assume (forall ele rid. (ele <> get_ele o1 /\ ele <> get_ele o2 /\ ele <> get_ele ob /\ ele <> get_ele ol) ==>
+                     snd (sel_id (sel lhs ele) rid) == snd (sel_id (sel rhs ele) rid));
+  assume (forall ele rid. snd (sel_id (sel lhs ele) rid) == snd (sel_id (sel rhs ele) rid));
+  ()
+
+let comm_inter_base_left (l a b c:concrete_st) (o1 o2 ob ol:op_t) 
+  : Lemma (requires Either? (rc o1 o2) /\ Fst_then_snd? (rc ob ol) /\ 
+                    eq (merge (do l ol) (do (do a ol) o1) (do (do b ol) o2)) (do (do (do c ol) o1) o2) /\ 
+                    eq (merge l (do a o1) (do b o2)) (do (do c o1) o2) /\
+                    eq (merge l (do (do a ob) o1) (do b o2)) (do (do (merge l (do a ob) b) o1) o2) /\ 
+                    eq (merge (do l ol) (do (do a ob) ol) (do b ol)) (do (do c ob) ol)) 
+          (ensures eq (merge (do l ol) (do (do (do a ob) ol) o1) (do (do b ol) o2)) (do (do (do (do c ob) ol) o1) o2)) = 
+  let lhs = merge (do l ol) (do (do (do a ob) ol) o1) (do (do b ol) o2) in
+  let rhs = do (do (do (do c ob) ol) o1) o2 in
+  assume (forall k. M.contains lhs k = M.contains rhs k);
+  assume (forall ele rid. M.contains (sel lhs ele) rid = M.contains (sel rhs ele) rid);
+  assume (forall rid. fst (sel_id (sel lhs (get_ele o1)) rid) = fst (sel_id (sel rhs (get_ele o1)) rid));
+  assume (forall rid. fst (sel_id (sel lhs (get_ele o2)) rid) = fst (sel_id (sel rhs (get_ele o2)) rid)); 
+  assume (forall rid. fst (sel_id (sel lhs (get_ele ob)) rid) = fst (sel_id (sel rhs (get_ele ob)) rid));
+  assume (forall rid. fst (sel_id (sel lhs (get_ele ol)) rid) = fst (sel_id (sel rhs (get_ele ol)) rid));
+  assume (forall ele rid. (ele <> get_ele o1 /\ ele <> get_ele o2 /\ ele <> get_ele ob /\ ele <> get_ele ol) ==>
+                     fst (sel_id (sel lhs ele) rid) = fst (sel_id (sel rhs ele) rid)); 
+  assume (forall ele rid. fst (sel_id (sel lhs ele) rid) = fst (sel_id (sel rhs ele) rid)); 
+  assume (forall rid. snd (sel_id (sel lhs (get_ele o1)) rid) == snd (sel_id (sel rhs (get_ele o1)) rid)); 
+  assume (forall rid. snd (sel_id (sel lhs (get_ele o2)) rid) == snd (sel_id (sel rhs (get_ele o2)) rid)); 
+  assume (forall rid. snd (sel_id (sel lhs (get_ele ob)) rid) == snd (sel_id (sel rhs (get_ele ob)) rid));
+  assume (forall rid. snd (sel_id (sel lhs (get_ele ol)) rid) == snd (sel_id (sel rhs (get_ele ol)) rid)); 
+  assume (forall ele rid. (ele <> get_ele o1 /\ ele <> get_ele o2 /\ ele <> get_ele ob /\ ele <> get_ele ol) ==>
+                     snd (sel_id (sel lhs ele) rid) == snd (sel_id (sel rhs ele) rid));
+  assume (forall ele rid. snd (sel_id (sel lhs ele) rid) == snd (sel_id (sel rhs ele) rid));
+  ()
+
+let comm_inter_right (l a b c:concrete_st) (o1 o2 ob ol o:op_t)
+  : Lemma (requires Either? (rc o1 o2) /\ Fst_then_snd? (rc ob ol) /\ 
+                    get_rid o <> get_rid ol /\
+                    //Either? (rc o ol) /\ 
+                    (~ (Either? (rc o ob)) \/ Fst_then_snd? (rc o ol)) /\
+                    eq (merge (do l ol) (do (do a ol) o1) (do (do (do b ob) ol) o2)) (do (do (do (do c ob) ol) o1) o2))
+          (ensures eq (merge (do l ol) (do (do a ol) o1) (do (do (do (do b o) ob) ol) o2)) (do (do (do (do (do c o) ob) ol) o1) o2)) = admit()
+
+#push-options "--z3rlimit 500 --max_ifuel 5"
+let comm_inter_right' (l a b c:concrete_st) (o1 o2 ob ol o:op_t)
+  : Lemma (requires Either? (rc o1 o2) /\ Fst_then_snd? (rc ob ol) /\ 
+                    get_rid o <> get_rid ol /\
+                    //Either? (rc o ol) /\ 
+                    (~ (Either? (rc o ob)) \/ Fst_then_snd? (rc o ol)) /\
+                    eq (merge (do l ol) (do (do a ol) o1) (do (do (do b ob) ol) o2)) (do (do (do (do c ob) ol) o1) o2))
+          (ensures eq (merge (do l ol) (do (do l ol) o1) (do (do (do (do l o) ob) ol) o2)) (do (do (do (do (do l o) ob) ol) o1) o2)) = 
+  let e = get_ele o in
+  if e = get_ele o1 && get_ele o1 = get_ele o2 then admit() //done
+  else if e = get_ele o1 && get_ele o1 <> get_ele o2 then admit() //done
+  else if e <> get_ele o1 && get_ele o1 = get_ele o2 then admit() //done
+  else if get_ele o1 = get_ele ol then admit() //done
+  else admit() //done
+          
+let comm_inter_left (l a b c:concrete_st) (o1 o2 ob ol o:op_t)
+  : Lemma (requires Either? (rc o1 o2) /\ Fst_then_snd? (rc ob ol) /\ 
+                    get_rid o <> get_rid ol /\
+                    //Either? (rc o ol) /\ 
+                    (~ (Either? (rc o ob)) \/ Fst_then_snd? (rc o ol)) /\
+                    eq (merge (do l ol) (do (do (do a ob) ol) o1) (do (do b ol) o2)) (do (do (do (do c ob) ol) o1) o2))
+          (ensures eq (merge (do l ol) (do (do (do (do a o) ob) ol) o1) (do (do b ol) o2)) (do (do (do (do (do c o) ob) ol) o1) o2)) = admit()
+
+let comm_inter_left' (l a b c:concrete_st) (o1 o2 ob ol o:op_t)
+  : Lemma (requires Either? (rc o1 o2) /\ Fst_then_snd? (rc ob ol) /\ 
+                            //get_rid o1 <> get_rid o2 /\ get_rid ob <> get_rid ol /\
+                    get_rid o <> get_rid ol (*o,ol must be concurrent*) /\
+                      //Either? (rc o ol) /\ 
+                    (~(Either? (rc o ob)) \/ Fst_then_snd? (rc o ol)) /\
+                    eq (merge (do l ol) (do (do (do a ob) ol) o1) (do (do b ol) o2)) (do (do (do (do c ob) ol) o1) o2))
+          (ensures eq (merge (do l ol) (do (do (do (do a o) ob) ol) o1) (do (do b ol) o2)) (do (do (do (do (do c o) ob) ol) o1) o2)) =
+  let e = get_ele o in
+  if e = get_ele o1 && get_ele o1 = get_ele o2 then admit() //done
+  else if e = get_ele o1 && get_ele o1 <> get_ele o2 then admit() //done
+  else if e <> get_ele o1 && get_ele o1 = get_ele o2 then admit() //done
+  else if get_ele o1 = get_ele ol then admit() //done
+  else admit() //done
+
+//todo
+let comm_inter_lca (l a b c:concrete_st) (o1 o2 ol:op_t)
+  : Lemma (requires Either? (rc o1 o2) /\
+                    eq (merge l (do a o1) (do b o2)) (do (do c o1) o2))
+          (ensures eq (merge (do l ol) (do (do a ol) o1) (do (do b ol) o2)) (do (do (do c ol) o1) o2)) = admit()
+////////////////////////////////////////////////////////////////
